src/Reflection/Conversion.v
@@ -1,0 +1,117 @@
+(** * Convert between interpretations of types *)
+Require Import Crypto.Reflection.Syntax.
+Require Import Crypto.Util.Notations Crypto.Util.Tactics.
+
+Local Open Scope expr_scope.
+
+Section language.
+  Context (base_type_code : Type).
+  Context (op : flat_type base_type_code -> flat_type base_type_code -> Type).
+  Section map.
+    Context (interp_base_type1 interp_base_type2 : base_type_code -> Type).
+    Context (f_const : forall t, interp_flat_type_gen interp_base_type1 t -> interp_flat_type_gen interp_base_type2 t).
+    Context {var1 var2 : base_type_code -> Type}.
+    Context (f_var12 : forall t, var1 t -> var2 t)
+            (f_var21 : forall t, var2 t -> var1 t).
+
+    Fixpoint mapf
+             {t}
+             (e : @exprf base_type_code interp_base_type1 op var1 t)
+      : @exprf base_type_code interp_base_type2 op var2 t
+      := match e in @exprf _ _ _ _ t return @exprf _ _ _ _ t with
+         | Const _ x => Const (f_const _ x)
+         | Var _ x => Var (f_var12 _ x)
+         | Op _ _ op args => Op op (@mapf _ args)
+         | LetIn _ ex _ eC => LetIn (@mapf _ ex)
+                               (fun x => @mapf _ (eC (mapf_interp_flat_type_gen base_type_code f_var21 x)))
+         | Pair _ ex _ ey => Pair (@mapf _ ex)
+                                 (@mapf _ ey)
+         end.
+
+    Fixpoint map {t} (e : @expr base_type_code interp_base_type1 op var1 t)
+      : @expr base_type_code interp_base_type2 op var2 t
+      := match e with
+         | Return _ x => Return (mapf x)
+         | Abs _ _ f => Abs (fun x => @map _ (f (f_var21 _ x)))
+         end.
+  End map.
+
+  Section mapf_id.
+    Context (functional_extensionality : forall {A B} (f g : A -> B), (forall x, f x = g x) -> f = g)
+            {interp_base_type : base_type_code -> Type}
+            {var : base_type_code -> Type}.
+
+    Lemma mapf_idmap_ext {t} e
+      : @mapf interp_base_type interp_base_type
+              (fun _ x => x)
+              var var
+              (fun _ x => x) (fun _ x => x)
+              t e
+        = e.
+    Proof.
+      induction e;
+        repeat match goal with
+               | _ => reflexivity
+               | _ => progress simpl in *
+               | _ => rewrite_hyp !*
+               | _ => apply (f_equal2 (fun x f => LetIn x f))
+               | _ => solve [ eauto ]
+               | _ => apply functional_extensionality; intro
+               end.
+      clear e IHe H.
+      revert dependent e0; revert dependent tC; revert dependent x; induction tx; simpl; [ reflexivity | ]; intros.
+      destruct x as [x0 x1]; simpl in *.
+      lazymatch goal with
+      | [ |- ?e0 (?x0', ?x1')%core = _ ]
+        => rewrite (IHtx1 x0 _ (fun x0'' => e0 (x0'', x1')%core)); cbv beta in *
+      end.
+      lazymatch goal with
+      | [ |- ?e0 (?x0', ?x1')%core = _ ]
+        => rewrite (IHtx2 x1 _ (fun x1'' => e0 (x0', x1'')%core)); cbv beta in *
+      end.
+      reflexivity.
+    Qed.
+  End mapf_id.
+
+  Section mapf_id_interp.
+    Context {interp_base_type : base_type_code -> Type}
+            (interp_op : forall src dst, op src dst -> interp_flat_type_gen interp_base_type src -> interp_flat_type_gen interp_base_type dst)
+            (f_const : forall t, interp_flat_type_gen interp_base_type t -> interp_flat_type_gen interp_base_type t)
+            (f_var12 f_var21 : forall t, interp_base_type t -> interp_base_type t)
+            (f_const_id : forall t x, f_const t x = x)
+            (f_var12_id : forall t x, f_var12 t x = x)
+            (f_var21_id : forall t x, f_var21 t x = x).
+
+    Lemma mapf_idmap {t} e
+      : interpf interp_op
+                (@mapf interp_base_type interp_base_type
+                       f_const
+                       _ _
+                       f_var12 f_var21
+                       t e)
+        = interpf interp_op e.
+    Proof.
+      induction e;
+        repeat match goal with
+               | _ => reflexivity
+               | _ => progress simpl in *
+               | _ => rewrite_hyp !*
+               | _ => apply (f_equal2 (fun x f => LetIn x f))
+               | _ => solve [ eauto ]
+               end.
+      clear H IHe.
+      generalize (interpf interp_op e); intro x; clear e.
+      revert dependent e0; revert dependent tC; revert dependent x; induction tx; simpl;
+        [ intros; rewrite_hyp ?*; reflexivity | ]; intros.
+      destruct x as [x0 x1]; simpl in *.
+      lazymatch goal with
+      | [ |- interpf _ (?e0 (?x0', ?x1')%core) = _ ]
+        => rewrite (IHtx1 x0 _ (fun x0'' => e0 (x0'', x1')%core)); cbv beta in *
+      end.
+      lazymatch goal with
+      | [ |- interpf _ (?e0 (?x0', ?x1')%core) = _ ]
+        => apply (IHtx2 x1 _ (fun x1'' => e0 (x0', x1'')%core)); cbv beta in *
+      end.
+    Qed.
+  End mapf_id_interp.
+End language.
